Examples/UniswapV2Pair/Mint.lean
@@ -1,0 +1,22 @@
+import Examples.UniswapV2Pair.Dispatch
+import Reasoning.Refinement
+
+open Solm ABI Ethereum Ethereum.EVM Reasoning.Theory Reasoning.Reach Reasoning.Refinement
+
+set_option maxRecDepth 2000000
+
+namespace UniswapV2Pair
+
+/-! ## `mint(address)` placeholder -/
+
+theorem uniswapMintBody
+    {cA gh bl σ_evm σ_solm σ₀ A I} {g : UInt256}
+    (hcode : I.code = uniswapV2PairBytecode) (hsize : I.calldata.size < UInt256.size)
+    (hperm : I.perm = true) (hwv : I.weiValue = ⟨0⟩)
+    (hsel : selIs I ⟨#[0x6a, 0x62, 0x78, 0x42]⟩)
+    (hdispatch : dispatchMsg contract I.calldata = some mintTransition)
+    (hAccounts : accountMapEquiv σ_evm σ_solm) :
+    runtimeEquivalenceFor config contract cA gh bl σ_evm σ_solm σ₀ g A I := by
+  sorry
+
+end UniswapV2Pair
