Examples/UniswapV2Pair/Symbol.lean
@@ -1,0 +1,21 @@
+import Examples.UniswapV2Pair.Dispatch
+import Reasoning.Refinement
+
+open Solm ABI Ethereum Ethereum.EVM Reasoning.Theory Reasoning.Reach Reasoning.Refinement
+
+set_option maxRecDepth 2000000
+
+namespace UniswapV2Pair
+
+/-! ## `symbol()` placeholder -/
+
+theorem uniswapSymbolBody
+    {cA gh bl σ_evm σ_solm σ₀ A I} {g : UInt256}
+    (hcode : I.code = uniswapV2PairBytecode) (hsize : I.calldata.size < UInt256.size)
+    (hwv : I.weiValue = ⟨0⟩) (hsel : selIs I ⟨#[0x95, 0xd8, 0x9b, 0x41]⟩)
+    (hdispatch : dispatchMsg contract I.calldata = some symbolTransition)
+    (hAccounts : accountMapEquiv σ_evm σ_solm) :
+    runtimeEquivalenceFor config contract cA gh bl σ_evm σ_solm σ₀ g A I := by
+  sorry
+
+end UniswapV2Pair
