Examples/UniswapV2Pair/TransferFromDecode.lean
@@ -55,4 +55,50 @@ theorem uniswapTransferFromBodyDecodeFailed_short
   exact uniswapTransferFromBodyCoreDecodeFailed_short hcode hsize hsz4 hshort hdispatch
     (uniswapReachTransferFromBody (g := Sat256.ofUInt256 g) hcode hwv hsz4 hsize hsel)
 
+theorem uniswapTransferFromBody
+    {cA gh bl σ_evm σ_solm σ₀ A I} {g : UInt256}
+    (hcode : I.code = uniswapV2PairBytecode) (hsize : I.calldata.size < UInt256.size)
+    (hperm : I.perm = true) (hwv : I.weiValue = ⟨0⟩)
+    (hsel : selIs I ⟨#[0x23, 0xb8, 0x72, 0xdd]⟩)
+    (hdispatch : dispatchMsg contract I.calldata = some transferFromTransition)
+    (hAccounts : accountMapEquiv σ_evm σ_solm) :
+    runtimeEquivalenceFor config contract cA gh bl σ_evm σ_solm σ₀ g A I := by
+  by_cases hsz100 : 100 ≤ I.calldata.size
+  · by_cases hbig : I.calldata.size < 2 ^ 255 + 4
+    · by_cases hcanonFrom : (transferFromFromWord I).toNat < EVM.addressModulus
+      · by_cases hcanonTo : (transferFromToWord I).toNat < EVM.addressModulus
+        · by_cases hmax : (transferFromCurrentAllowanceWord
+            (initState cA gh bl σ_evm σ₀ (Sat256.ofUInt256 g) A I) I).toNat =
+              UInt256.size - 1
+          · by_cases hbalance : (transferFromValueWord I).toNat ≤
+              (transferFromFromBalanceWord
+                (initState cA gh bl σ_evm σ₀ (Sat256.ofUInt256 g) A I) I).toNat
+            · by_cases hfit : transferFromNewToNatMax
+                (initState cA gh bl σ_evm σ₀ (Sat256.ofUInt256 g) A I) I <
+                  UInt256.size
+              · exact uniswapTransferFromBodyOk_maxAllowance hcode hsize hperm hwv hsel
+                  hsz100 hbig hcanonFrom hcanonTo hmax hbalance hfit hdispatch hAccounts
+              · sorry
+            · sorry
+          · by_cases hallowance : (transferFromValueWord I).toNat ≤
+              (transferFromCurrentAllowanceWord
+                (initState cA gh bl σ_evm σ₀ (Sat256.ofUInt256 g) A I) I).toNat
+            · by_cases hbalance : (transferFromValueWord I).toNat ≤
+                (transferFromFromBalanceWord (transferFromAfterAllowanceState
+                  (initState cA gh bl σ_evm σ₀ (Sat256.ofUInt256 g) A I) I) I).toNat
+              · by_cases hfit : transferFromNewToNat
+                  (initState cA gh bl σ_evm σ₀ (Sat256.ofUInt256 g) A I) I <
+                    UInt256.size
+                · exact uniswapTransferFromBodyOk_finiteAllowance hcode hsize hperm hwv
+                    hsel hsz100 hbig hcanonFrom hcanonTo hmax hallowance hbalance hfit
+                    hdispatch hAccounts
+                · sorry
+              · sorry
+            · sorry
+        · sorry
+      · sorry
+    · sorry
+  · exact uniswapTransferFromBodyDecodeFailed_short hcode hsize hwv hsel (by omega)
+      hdispatch
+
 end UniswapV2Pair
